cfg example

autth/test.lean
@@ -3,6 +3,7 @@ import Mathlib.Data.Set.Function
 import Mathlib.Tactic
 import Mathlib.Data.List.Join
 import Mathlib.Util.Delaborators
+import Mathlib.Computability.ContextFreeGrammar
 
 import Mathlib.Computability.EpsilonNFA
 
@@ -26,11 +27,11 @@ namespace PDA
 def step {Q T S : Type} {pda : PDA Q T S} (r₁ : PDA_id pda) : Set (PDA_id pda) :=
   match r₁ with
     | ⟨q,a::w,Z::α⟩ =>
-        {r₂ : PDA_id pda | ∃ p:Q, ∃β:List S, (p,β) ∈ pda.transition_fun q a Z ∧
+        {r₂ : PDA_id pda | ∃ (p:Q) (β:List S), (p,β) ∈ pda.transition_fun q a Z ∧
                           r₂=⟨p, w, (β ++ α)⟩ } ∪
-        {r₂ : PDA_id pda | ∃p:Q, ∃β:List S, (p,β) ∈ pda.transition_fun' q Z ∧
+        {r₂ : PDA_id pda | ∃(p:Q)(β:List S), (p,β) ∈ pda.transition_fun' q Z ∧
                           r₂=⟨p, a :: w, (β ++ α)⟩}
-    | ⟨q,Nil,Z::α⟩ => {r₂ : PDA_id pda | ∃p:Q, ∃β:List S, (p,β) ∈ pda.transition_fun' q Z ∧
+    | ⟨q,Nil,Z::α⟩ => {r₂ : PDA_id pda | ∃(p:Q)(β:List S), (p,β) ∈ pda.transition_fun' q Z ∧
                                          r₂=⟨p, Nil, (β ++ α)⟩}
     | ⟨q,w,Nil⟩ => {r₂ : PDA_id pda | r₂ = ⟨q,w,Nil⟩} -- Empty stack
 
@@ -42,8 +43,13 @@ def stepSetN {Q T S : Type} {pda : PDA Q T S} (n : ℕ) (R : Set (PDA_id pda))  
   | 0 => R
   | Nat.succ m => stepSet (stepSetN m R)
 
+
 /-def stepRel {Q T S : Type} {pda : PDA Q T S} (r₁ : PDA_id pda)(r₂ : PDA_id pda) : Prop :=
   r₂ ∈ step r₁-/
+
+inductive stepRel' {Q T S : Type} {pda : PDA Q T S}  : PDA_id pda→ PDA_id pda→Prop :=
+  | base : (r₁ : PDA_id pda) → stepRel' r₁ r₁
+  | step : {r₁ r' r₂ : PDA_id pda} → (r'∈ step r₁) → (stepRel' r' r₂) → stepRel' r₁ r₂
 
 def stepRelN {Q T S : Type} {pda : PDA Q T S} (n : ℕ) (r₁ : PDA_id pda)(r₂ : PDA_id pda) : Prop :=
   r₂ ∈ stepSetN n {r₁}
@@ -58,3 +64,54 @@ def acceptsByEmptyStack {Q T S : Type} (pda : PDA Q T S) : Language T :=
 def acceptsByFinalState {Q T S : Type} (pda : PDA Q T S) : Language T :=
   {w : List T | ∃q ∈ pda.final_states,∃ γ:List S,
       stepRel (⟨pda.initial_state, w, [pda.start_symbol]⟩ : PDA_id pda) ⟨q,[],γ⟩ }
+
+
+inductive alph where
+  | a
+  | b
+
+inductive nt where
+  | S
+
+open alph
+open nt
+open Symbol
+open ContextFreeGrammar
+
+def G : ContextFreeGrammar alph := ⟨nt,S,
+  [⟨S,[]⟩,
+  ⟨nt.S,[terminal a, nonterminal S, terminal b]⟩]⟩
+
+example : [a,a,b,b] ∈ G.language := by
+  rw [mem_language_iff]
+  simp
+  rw [Derives]
+  apply Relation.ReflTransGen.tail
+  case b => exact [terminal a,terminal a,nonterminal S, terminal b,terminal b]
+  case a =>
+    apply Relation.ReflTransGen.tail
+    case b => exact [terminal a,nonterminal S,terminal b]
+    case a =>
+      apply Relation.ReflTransGen.tail
+      case b => exact [nonterminal S]
+      case a => rw [ (by rfl :G.initial = S)]
+      case a =>
+        use ⟨nt.S,[terminal a, nonterminal S, terminal b]⟩
+        constructor
+        · simp [G]
+        · apply (ContextFreeRule.rewrites_iff [nonterminal S] [terminal a, nonterminal S, terminal b]).mpr
+          use []
+          use []
+          simp
+    case a =>
+      use ⟨nt.S,[terminal a, nonterminal S, terminal b]⟩
+      constructor
+      · simp [G]
+      · apply ContextFreeRule.Rewrites.cons (terminal a)
+        apply ContextFreeRule.Rewrites.head [terminal b]
+  case a =>
+    use ⟨nt.S,[]⟩
+    simp [G]
+    apply ContextFreeRule.Rewrites.cons (terminal a)
+    apply ContextFreeRule.Rewrites.cons (terminal a)
+    apply ContextFreeRule.Rewrites.head [terminal b, terminal b]
